src/TV/seop_llvmop.v
@@ -615,7 +615,7 @@ Case "dbInsertValue".
 Case "dbMalloc".
   inversion H; subst. clear H. 
   exists l0. exists ps. exists cs. exists tmn0.
-  exists (updateAddAL _ lc0 id0 (ptr2GV TD0 (mb, 0))). exists als0. exists Mem'.
+  exists (updateAddAL _ lc0 id0 (blk2GV TD0 mb)). exists als0. exists Mem'.
   exists cs1. split; auto.
   right. left.
   exists (insn_malloc id0 t sz0 align0).
@@ -633,7 +633,7 @@ Case "dbFree".
 Case "dbAlloca".
   inversion H; subst. clear H.
   exists l0. exists ps. exists cs. exists tmn0.
-  exists (updateAddAL _ lc0 id0 (ptr2GV TD0 (mb, 0))). exists (mb::als0). exists Mem'.
+  exists (updateAddAL _ lc0 id0 (blk2GV TD0 mb)). exists (mb::als0). exists Mem'.
   exists cs1. split; auto.
   right. left.
   exists (insn_alloca id0 t sz0 align0).
@@ -696,7 +696,7 @@ Case "dbIcmp".
 Case "dbSelect".
   inversion H; subst. clear H.
   exists l0. exists ps. exists cs. exists tmn0.
-  exists (if c then updateAddAL _ lc0 id0 gv2 else updateAddAL _ lc0 id0 gv1). exists als0. exists Mem1.
+  exists (if Coqlib.zeq c 0 then updateAddAL _ lc0 id0 gv2 else updateAddAL _ lc0 id0 gv1). exists als0. exists Mem1.
   exists cs1. split; auto.
   right. left.
   exists (insn_select id0 v0 t v1 v2).
