src/TV/symexe_sound.v
@@ -139,7 +139,7 @@ Proof.
     inversion malloc_denotes_gv'; subst.
     apply smem_denotes_mem_det with (Mem2:=Mem1) in H10; auto.
     subst.
-    exists (updateAddAL _ lc i0 (ptr2GV TD (mb, 0))). exists als. exists Mem5. exists trace_nil.
+    exists (updateAddAL _ lc i0 (blk2GV TD mb)). exists als. exists Mem5. exists trace_nil.
     split; eauto.
 
   Case "insn_free".
@@ -162,7 +162,7 @@ Proof.
     inversion alloca_denotes_gv'; subst.
     apply smem_denotes_mem_det with (Mem2:=Mem1) in H10; auto.
     subst.
-    exists (updateAddAL _ lc i0 (ptr2GV TD (mb, 0))). exists (mb::als). exists Mem5. exists trace_nil.
+    exists (updateAddAL _ lc i0 (blk2GV TD mb)). exists (mb::als). exists Mem5. exists trace_nil.
     split; eauto.
 
   Case "insn_load".
@@ -265,7 +265,7 @@ Proof.
     apply value2Sterm_denotes__implies__genericvalue with (lc:=lc)(gl:=gl) in H5; auto.
     apply value2Sterm_denotes__implies__genericvalue with (lc:=lc)(gl:=gl) in H10; auto.
     apply value2Sterm_denotes__implies__genericvalue with (lc:=lc)(gl:=gl) in H12; auto.
-    exists (if c0 then updateAddAL _ lc i0 gv2 else updateAddAL _ lc i0 gv1). exists als. exists Mem1. exists trace_nil. 
+    exists (if Coqlib.zeq c0 0 then updateAddAL _ lc i0 gv2 else updateAddAL _ lc i0 gv1). exists als. exists Mem1. exists trace_nil. 
     assert (getOperandInt TD 1 v lc gl = Some c0) as J.
       unfold getOperandInt. rewrite H5. auto.
     split; eauto.
