src/ssa/compcert/Memdata.v
@@ -16,6 +16,7 @@
 
 (** In-memory representation of values. *)
 
+Require Import Znumtheory.
 Require Import Coqlib.
 Require Import AST.
 Require Import Integers.
