src/ssa/llvm_op/ssa_interpreter.v
@@ -147,7 +147,7 @@ Definition switchToNewBasicBlock (Dest:block) (PrevBB:block) (Values:Mem): (bloc
 Definition getOperandValue (v:value) (Values:Mem) : option GenericValue := 
 match v with
 | value_id id => Values id
-| value_const (const_int _ n) => Some (GenericValue_int n)
+| value_const (const_int _ n) => Some (GenericValue_int 0)
 | value_const (const_undef _) => Some (GenericValue_int 0)
 | _ => None
 end.
